src/base/recovery_adequacy.v
@@ -1,0 +1,628 @@
+From iris.proofmode Require Import tactics.
+From iris.algebra Require Import gmap auth agree gset coPset.
+From Perennial.Helpers Require Import ipm.
+From Perennial.base_logic.lib Require Import wsat.
+From Perennial.program_logic Require Export weakestpre.
+From Perennial.program_logic Require Export crash_lang.
+From Perennial.program_logic Require Import crash_adequacy.
+Import uPred.
+
+From self.nextgen Require Import nextgen_promises.
+From self.base Require Export recovery_weakestpre.
+
+Set Default Proof Using "Type".
+Set Default Goal Selector "!".
+
+Section recovery_adequacy.
+  Context {Σ} {Ω : gGenCmras Σ} `{!irisGS Λ Σ, !generationGS Λ Σ}.
+  Implicit Types s : stuckness.
+  Implicit Types P : iProp Σ.
+  Implicit Types Φ : val Λ → iProp Σ.
+  Implicit Types Φinv : iProp Σ.
+  Implicit Types Φr : val Λ → iProp Σ.
+  Implicit Types v : val Λ.
+  Implicit Types e : expr Λ.
+
+  Notation wptp s t := ([∗ list] ef ∈ t, WPC ef @ s; ⊤ {{ fork_post }} {{ True }})%I.
+
+  Notation steps_sum := crash_adequacy.steps_sum.
+
+  (* The assertion [P] holds after [lenght ns] crashes where each execution is
+  [ns !! i] many steps. *)
+  (* NOTE: We probably need a nextgen modality in here. *)
+  Fixpoint step_fupdN_fresh ncurrent (ns: list nat)
+           (P : iProp Σ) {struct ns} :=
+    match ns with
+    | [] => P
+    | (n :: ns) =>
+      (£ (steps_sum (num_laters_per_step) (step_count_next) ncurrent (S n)) -∗
+        ||={⊤|⊤,∅|∅}=> ||▷=>^(steps_sum (num_laters_per_step) (step_count_next)
+                                       ncurrent (S n)) ||={∅|∅, ⊤|⊤}=>
+       ||={⊤|⊤,∅|∅}=> ||▷=>^2 ||={∅|∅, ⊤|⊤}=> ⚡==>
+       |={⊤}=>
+         step_fupdN_fresh ((Nat.iter (S n) step_count_next ncurrent)) ns P)
+    end%I.
+
+  Lemma step_fupdN_fresh_wand ncurr1 ncurr2 (ns: list nat) Q Q':
+    ncurr1 = ncurr2 →
+    step_fupdN_fresh ncurr1 (ns) Q -∗ (Q -∗ Q')
+    -∗ step_fupdN_fresh ncurr2 ns Q'.
+  Proof.
+  Admitted.
+  (*   revert ncurr1 ncurr2. *)
+  (*   induction ns => ?? Hncurr. *)
+  (*   - iIntros "H Hwand". iApply "Hwand". eauto. *)
+  (*   - iIntros "H Hwand Hlc". rewrite /step_fupdN_fresh -/step_fupdN_fresh. *)
+  (*     rewrite {1}Hncurr. *)
+  (*     iSpecialize ("H" with "Hlc"). *)
+  (*     iApply (step_fupd2N_inner_wand with "H"); try auto. *)
+  (*     { subst. auto. } *)
+  (*     iIntros "H". *)
+  (*     iMod "H". iModIntro. iApply (step_fupd2N_wand with "H"). iIntros "H". *)
+  (*     iMod "H". iModIntro. *)
+  (*     iMod "H" as "H". *)
+  (*     iModIntro. iApply (IHns with "H"). *)
+  (*     { subst. auto. } *)
+  (*     eauto. *)
+  (* Qed. *)
+
+  Lemma wptp_recv_strong_normal_adequacy {CS Φ Φinv Φr κs' s} n ncurr mj D r1 e1 t1 κs t2 σ1 g1 σ2 g2 :
+    nrsteps (CS := CS) r1 [n] (e1 :: t1, (σ1,g1)) κs (t2, (σ2,g2)) Normal →
+    state_interp σ1 (length t1) -∗
+    global_state_interp g1 ncurr mj D (κs ++ κs') -∗
+    wpr CS s ⊤ e1 r1 Φ Φinv Φr -∗
+    wptp s t1 -∗ (
+      (£ (steps_sum num_laters_per_step step_count_next ncurr n) -∗
+       ||={⊤|⊤,∅|∅}=> ||▷=>^(steps_sum num_laters_per_step step_count_next ncurr n) ||={∅|∅,⊤|⊤}=>
+      ∃ e2 t2',
+      ⌜ t2 = e2 :: t2' ⌝ ∗
+      state_interp σ2 (length t2') ∗
+      global_state_interp g2 (Nat.iter n step_count_next ncurr) mj D κs' ∗
+      from_option Φ True (to_val e2) ∗
+      ([∗ list] v ∈ omap to_val t2', fork_post v))).
+  Proof.
+    iIntros (Hstep) "Hσ Hg He Ht".
+    inversion Hstep. subst.
+    iPoseProof (wptp_strong_adequacy with "Hσ Hg [He] Ht") as "H".
+    { eauto. }
+    {rewrite wpr_unfold /wpr_pre. iApply "He". }
+    iSpecialize ("H" with "[]"). { admit. }
+    rewrite /step_fupdN_fresh.
+    iIntros "Hlc". iSpecialize ("H" with "Hlc").
+    iApply (step_fupd2N_wand with "H"); auto.
+  Admitted.
+
+  Lemma wptp_recv_normal_progress {CS Φ Φinv Φr κs'} n ns ncurr mj D r1 e1 t1 κs t2 σ1 g1 σ2 g2 e2 :
+    nrsteps (CS := CS) r1 (ns ++ [n]) (e1 :: t1, (σ1,g1)) κs (t2, (σ2,g2)) Normal →
+    e2 ∈ t2 →
+    state_interp σ1 (length t1) -∗
+    global_state_interp g1 ncurr mj D (κs ++ κs') -∗
+    wpr CS NotStuck ⊤ e1 r1 Φ Φinv Φr -∗
+    wptp NotStuck t1 -∗ step_fupdN_fresh ncurr ns (
+      (* ⌜ HG' = ⌝ ∗ *)
+    (£ (steps_sum num_laters_per_step step_count_next ncurr (S n)) -∗
+     ||={⊤|⊤,∅|∅}=> ||▷=>^(steps_sum num_laters_per_step step_count_next ncurr n) ||={∅|∅, ∅|∅}=>
+     ||▷=>^(num_laters_per_step (Nat.iter n step_count_next ncurr) + 1)
+          ⌜ not_stuck e2 σ2 g2 ⌝ )).
+  Proof.
+    iIntros (Hstep Hel) "Hσ Hg He Ht".
+    inversion Hstep. subst.
+    iPoseProof (wptp_progress with "Hσ Hg [He] Ht") as "H".
+    { eauto. } { done. }
+    {rewrite wpr_unfold /wpr_pre. iApply "He". }
+    iSpecialize ("H" with "[]"). { admit. }
+    assert (ns = []) as ->;
+      first by (eapply nrsteps_normal_empty_prefix; eauto).
+    inversion H. subst.
+    rewrite /step_fupdN_fresh.
+    (* iSplitL ""; first by eauto. *)
+    iIntros "Hlc". iSpecialize ("H" with "Hlc").
+    iApply (step_fupd2N_wand with "H"); auto.
+  Admitted.
+
+  Fixpoint sum_crash_steps ns :=
+    match ns with
+    | [] => 0
+    | n :: ns => (S n) + (sum_crash_steps ns)
+    end.
+
+  Lemma wptp_recv_strong_crash_adequacy {CS Φ Φinv Φinv' Φr κs' s} ncurr mj D ns n r1 e1 t1 κs t2 σ1 g1 σ2 g2 :
+    nrsteps (CS := CS) r1 (ns ++ [n]) (e1 :: t1, (σ1,g1)) κs (t2, (σ2,g2)) Crashed →
+    state_interp σ1 (length t1) -∗
+    global_state_interp g1 ncurr mj D (κs ++ κs') -∗
+    wpr CS s ⊤ e1 r1 Φ Φinv Φr -∗
+    ■ (Φinv -∗ □ Φinv') -∗
+    wptp s t1 -∗ (* NC 1 -∗ *) step_fupdN_fresh ncurr ns (
+      let ntot := (steps_sum num_laters_per_step step_count_next
+                             (Nat.iter (sum_crash_steps ns) step_count_next ncurr )
+                             n)  in
+      let ntot' := ((Nat.iter (n + sum_crash_steps ns) step_count_next ncurr)) in
+      £ ntot -∗
+      (||={⊤|⊤, ∅|∅}=> ||▷=>^ntot ||={∅|∅, ⊤|⊤}=> (∃ e2 t2',
+      ⌜ t2 = e2 :: t2' ⌝ ∗
+      state_interp σ2 (length t2') ∗
+      global_state_interp g2 ntot' mj D κs' ∗
+      from_option (Φr) True (to_val e2) ∗
+      □ Φinv' ∗
+      ([∗ list] v ∈ omap to_val t2', fork_post v)
+      (* ∗ NC 1 *)
+      ))).
+  Proof.
+    revert e1 t1 κs κs' t2 σ1 g1 ncurr σ2 Φ.
+    induction ns as [|n' ns' IH] => e1 t1 κs κs' t2 σ1 g1 ncurr σ2 Φ.
+    { rewrite app_nil_l.
+      inversion 1.
+      match goal with
+      | [ H : nrsteps _ _ _ _ _ _ |- _ ] => inversion H
+      end.
+    }
+    iIntros (Hsteps) "Hσ Hg He #Hinv Ht".
+    inversion_clear Hsteps as [|?? [t1' ?] ????? s0].
+    rewrite {1}/step_fupdN_fresh -/step_fupdN_fresh.
+    destruct ρ2 as (?&[σ2_pre_crash g2_pre_crash]).
+    rewrite -assoc wpr_unfold /wpr_pre.
+    rewrite Nat.iter_succ.
+    iIntros "Hlc".
+    iPoseProof (@wptp_strong_crash_adequacy with "[$] [$] [$] [$] [] [$]") as "H"; eauto.
+    { admit. }
+    iMod "H". iModIntro.
+    iApply (step_fupd2N_wand (steps_sum num_laters_per_step step_count_next ncurr (S n'))
+              with "H").
+    iIntros "H".
+    iMod "H".
+    iModIntro. iMod (fupd2_mask_subseteq ∅ ∅) as "Hclo"; [set_solver+..|].
+    iModIntro. iModIntro. iNext.
+    iMod ("Hclo") as "_".
+    iMod (fupd2_mask_subseteq ∅ ∅) as "Hclo"; [set_solver+..|].
+    iMod ("Hclo") as "_".
+    iDestruct "H" as (e2 t2' ?) "(H&Hσ&Hg&HC)".
+    iMod ("H" with "[//] Hσ Hg") as "H".
+    iMod (fupd2_mask_subseteq ∅ ∅) as "Hclo"; [set_solver+..|]. do 2 iModIntro. iNext.
+    iModIntro.
+    iMod ("Hclo") as "_".
+    iModIntro.
+    iModIntro.
+    destruct s0.
+    - iMod "H" as "(Hσ&Hg&Hr)".
+      iDestruct "Hr" as "(_&Hr)".
+      simpl in *.
+      iPoseProof (IH with "[Hσ] [Hg] Hr [] []") as "H"; eauto.
+      (* iExists _. *)
+      iModIntro. simpl. eauto.
+      iApply (step_fupdN_fresh_wand with "H").
+      { auto. }
+      iIntros "H Hlc".
+      iSpecialize ("H" with "[Hlc]").
+      { iExactEq "Hlc". f_equal.
+        rewrite {1}Nat.add_comm ?Nat.iter_add.
+        f_equal. rewrite -Nat.iter_succ -Nat.iter_succ_r //. }
+      iMod "H". iModIntro.
+      iEval rewrite -Nat.iter_succ Nat.iter_succ_r.
+      iApply step_fupd2N_le; last iApply (step_fupd2N_wand with "H").
+      { apply Nat.eq_le_incl. f_equal.
+        rewrite {1}Nat.add_comm ?Nat.iter_add.
+        f_equal. rewrite -Nat.iter_succ -Nat.iter_succ_r //. }
+      iIntros ">H".
+      rewrite {1}Nat.add_comm ?Nat.iter_add.
+      iDestruct "H" as (?? Heq) "(H1&Hg&?&?)".
+      iExists _, _. iFrame "∗".
+      iSplitL ""; first eauto.
+      iMod (global_state_interp_le with "Hg") as "$".
+      { apply Nat.eq_le_incl.
+        rewrite -?Nat.iter_succ_r -?Nat.iter_add Nat.add_assoc.
+        f_equal. lia. }
+      iModIntro; done.
+    - iMod "H" as "(Hσ&Hg&Hr)".
+      (* iExists HG'. *)
+      iAssert (□Φinv')%I as "#Hinv'".
+      { iDestruct "Hr" as "(Hr&_)".
+        iApply "Hinv". eauto.
+      }
+      iDestruct "Hr" as "(_&Hr)".
+      assert (ns' = []) as ->; first by (eapply nrsteps_normal_empty_prefix; eauto).
+      iDestruct (wptp_recv_strong_normal_adequacy with "[Hσ] [Hg] [Hr] []") as "H"; eauto.
+      iModIntro.
+      iIntros "Hlc".
+      simpl.
+      iSpecialize ("H" with "[Hlc]").
+      { iExactEq "Hlc". f_equal. rewrite Nat.add_0_r. done. }
+      iApply (step_fupd2N_inner_wand with "H"); try set_solver+.
+      { rewrite Nat.add_0_r. auto. }
+      iIntros "H".
+      iFrame "Hinv'". rewrite Nat.add_0_r.
+      rewrite -Nat.iter_succ Nat.iter_succ_r.
+      rewrite Nat.iter_add Nat.iter_succ_r.
+      eauto.
+  Admitted.
+
+  (* unfortunately this duplicates the large induction above.
+  There is probably some way to factor this... *)
+  Lemma wptp_recv_crash_progress {CS Φ Φinv Φinv' Φr κs'} ncurr mj D ns n r1 e1 t1 κs t2 σ1 g1 σ2 g2 ee2 :
+    nrsteps (CS := CS) r1 (ns ++ [n]) (e1 :: t1, (σ1,g1)) κs (t2, (σ2,g2)) Crashed →
+    ee2 ∈ t2 →
+    state_interp σ1 (length t1) -∗
+    global_state_interp g1 ncurr mj D (κs ++ κs') -∗
+    wpr CS NotStuck ⊤ e1 r1 Φ Φinv Φr -∗
+    ■ (Φinv -∗ □ Φinv') -∗
+    wptp NotStuck t1 -∗ (* NC 1-∗ *) step_fupdN_fresh ncurr ns (
+      let ntot := (steps_sum num_laters_per_step step_count_next
+                             (Nat.iter (sum_crash_steps ns) step_count_next ncurr )
+                             n)  in
+      let ntot' := ((Nat.iter (n + sum_crash_steps ns) step_count_next ncurr)) in
+      £ (ntot + num_laters_per_step ntot' + 1) -∗
+      (||={⊤|⊤, ∅|∅}=> ||▷=>^ntot ||={∅|∅, ∅|∅}=> ||▷=>^(num_laters_per_step ntot' + 1)
+      ⌜ not_stuck ee2 σ2 g2 ⌝)).
+  Proof.
+    revert e1 t1 κs κs' t2 σ1 g1 ncurr σ2 Φ.
+    induction ns as [|n' ns' IH] => e1 t1 κs κs' t2 σ1 g1 ncurr σ2 Φ.
+    { rewrite app_nil_l.
+      inversion 1.
+      match goal with
+      | [ H : nrsteps _ _ _ _ _ _ |- _ ] => inversion H
+      end.
+    }
+    iIntros (Hsteps Hel) "Hσ Hg He #Hinv Ht".
+    inversion_clear Hsteps as [|?? [t1' ?] ????? s0].
+    rewrite {1}/step_fupdN_fresh -/step_fupdN_fresh.
+    destruct ρ2 as (?&[σ2_pre_crash g2_pre_crash]).
+    rewrite -assoc wpr_unfold /wpr_pre.
+    rewrite Nat.iter_succ.
+    iIntros "Hlc".
+    iPoseProof (@wptp_strong_crash_adequacy with "[$] [$] [$] [$] [] [$]") as "H"; eauto.
+    { admit. }
+    iMod "H". iModIntro.
+    iApply (step_fupd2N_wand (steps_sum num_laters_per_step step_count_next ncurr (S n'))
+              with "H").
+    iIntros "H".
+    iMod "H".
+    iModIntro. iMod (fupd2_mask_subseteq ∅ ∅) as "Hclo"; [set_solver+..|].
+    iModIntro. iModIntro. iNext.
+    iMod ("Hclo") as "_".
+    iMod (fupd2_mask_subseteq ∅ ∅) as "Hclo"; [set_solver+..|].
+    iMod ("Hclo") as "_".
+    iDestruct "H" as (e2 t2' ?) "(H&Hσ&Hg&HC)".
+    iMod ("H" with "[//] Hσ Hg") as "H".
+    iMod (fupd2_mask_subseteq ∅ ∅) as "Hclo"; [set_solver+..|]. do 2 iModIntro. iNext.
+    iModIntro.
+    iMod ("Hclo") as "_".
+    iModIntro.
+    iModIntro.
+    destruct s0.
+    - iMod "H" as "(Hσ&Hg&Hr)".
+      iDestruct "Hr" as "(_&Hr)".
+      simpl in *.
+      iPoseProof (IH with "[Hσ] [Hg] Hr [] []") as "H"; eauto.
+      iModIntro. simpl. eauto.
+      iApply (step_fupdN_fresh_wand with "H").
+      { auto. }
+      iIntros "H Hlc".
+      iSpecialize ("H" with "[Hlc]").
+      { iExactEq "Hlc". f_equal. f_equal. f_equal.
+        - rewrite {1}Nat.add_comm ?Nat.iter_add.
+          f_equal. rewrite -Nat.iter_succ -Nat.iter_succ_r //.
+        - rewrite -?Nat.iter_succ_r -?Nat.iter_add.
+          f_equal. f_equal. lia. }
+      iMod "H". iModIntro.
+      iEval rewrite -Nat.iter_succ Nat.iter_succ_r.
+      iApply step_fupd2N_le; last iApply (step_fupd2N_wand with "H").
+      { apply Nat.eq_le_incl. f_equal.
+        rewrite {1}Nat.add_comm ?Nat.iter_add.
+        f_equal. rewrite -Nat.iter_succ -Nat.iter_succ_r //. }
+      iIntros ">H".
+      rewrite {1}[n + _]Nat.add_comm ?Nat.iter_add.
+      iModIntro. iApply (step_fupd2N_le with "H"); auto.
+      apply Nat.eq_le_incl. f_equal.
+      rewrite -?Nat.iter_succ_r -?Nat.iter_add Nat.add_assoc.
+      f_equal. lia.
+    - iMod "H" as "(Hσ & Hg & Hr)".
+      iAssert (□Φinv')%I as "#Hinv'".
+      { iDestruct "Hr" as "(Hr&_)".
+        iApply "Hinv". eauto.
+      }
+      iDestruct "Hr" as "(_&Hr)".
+      iDestruct (wptp_recv_normal_progress with "[Hσ] [Hg] [Hr] []") as "H"; eauto.
+      iApply (step_fupdN_fresh_wand with "H").
+      { simpl. lia. }
+      iModIntro.
+      iIntros "H".
+      (* iDestruct "H" as (->) "H". *)
+      rewrite steps_sum_S_r.
+      (* iClear "HC". *)
+      simpl.
+      assert (ns' = []) as ->; first by (eapply nrsteps_normal_empty_prefix; eauto).
+      iIntros "Hlc".
+      iSpecialize ("H" with "[Hlc]").
+      { simpl. rewrite Nat.add_0_r. iExactEq "Hlc". f_equal.
+        rewrite -assoc. f_equal.
+        rewrite ![_ + 1]comm. f_equal.
+        rewrite -Nat.iter_succ Nat.iter_succ_r.
+        rewrite Nat.iter_add Nat.iter_succ_r. done. }
+      simpl. iMod "H".
+      iApply (step_fupd2N_inner_wand with "H"); try set_solver+.
+      { rewrite Nat.add_0_r. auto. }
+      iIntros "H".
+      rewrite Nat.add_0_r.
+      rewrite -Nat.iter_succ Nat.iter_succ_r.
+      rewrite ![_ + 1]comm. simpl.
+      rewrite Nat.iter_add Nat.iter_succ_r.
+      eauto.
+  Admitted.
+
+  Lemma wptp_recv_strong_adequacy {CS Φ Φinv Φinv' Φr κs' s} ns mj D n r1 e1 t1 κs t2 σ1 g1 ncurr σ2 g2 stat :
+    nrsteps (CS := CS) r1 (ns ++ [n]) (e1 :: t1, (σ1,g1)) κs (t2, (σ2,g2)) stat →
+    state_interp σ1 (length t1) -∗
+    global_state_interp g1 ncurr mj D (κs ++ κs') -∗
+    wpr CS s ⊤ e1 r1 Φ Φinv Φr -∗
+    ■ (Φinv -∗ □ Φinv') -∗
+    wptp s t1 -∗ (* NC 1-∗ *) step_fupdN_fresh ncurr ns (
+      let ntot := (steps_sum num_laters_per_step step_count_next
+                             (Nat.iter (sum_crash_steps ns) step_count_next ncurr )
+                             n)  in
+      let ntot' := ((Nat.iter (n + sum_crash_steps ns) step_count_next ncurr)) in
+      £ ntot -∗
+      (||={⊤|⊤, ∅|∅}=> ||▷=>^ntot ||={∅|∅, ⊤|⊤}=> (∃ e2 t2',
+      ⌜ t2 = e2 :: t2' ⌝ ∗
+      state_interp σ2 (length t2') ∗
+      global_state_interp g2 ntot' mj D κs' ∗
+      (match stat with
+       | Normal => from_option Φ True (to_val e2)
+       | Crashed => from_option (Φr) True (to_val e2) ∗ □ Φinv'
+       end)  ∗
+      ([∗ list] v ∈ omap to_val t2', fork_post v)
+      (* ∗ NC 1 *)
+      ))).
+  Proof.
+    intros. destruct stat.
+    - iIntros.
+      iDestruct (wptp_recv_strong_crash_adequacy with "[$] [$] [$] [$] [$]") as "H"; eauto.
+      iApply (step_fupdN_fresh_wand with "H"); first auto.
+      iIntros "H Hlc". iSpecialize ("H" with "Hlc").
+      iApply (step_fupd2N_wand with "H"); auto.
+      iIntros "H".
+      iMod "H" as (???) "(?&H&?&?&?)". iExists _, _.
+      repeat (iSplitL ""; try iFrame; eauto).
+    - iIntros.
+      assert (ns = []) as ->; first by (eapply nrsteps_normal_empty_prefix; eauto).
+      iDestruct (wptp_recv_strong_normal_adequacy with "[$] [$] [$] [$]") as "H"; eauto.
+      iIntros "Hlc".
+      simpl. rewrite Nat.add_0_r. iSpecialize ("H" with "Hlc").
+      iMod "H". iModIntro.
+      iApply (step_fupd2N_wand with "H"); auto.
+      (* iIntros "H". *)
+      (* iMod "H" as (???) "(?&H&?&?&?)". iExists _, _. *)
+      (* iSplitL ""; first eauto. iFrame. eauto. *)
+  Qed.
+
+  Lemma wptp_recv_progress {CS Φ Φinv Φinv' Φr κs'} ns mj D n r1 e1 t1 κs t2 σ1 g1 ncurr σ2 g2 stat e2 :
+    nrsteps (CS := CS) r1 (ns ++ [n]) (e1 :: t1, (σ1,g1)) κs (t2, (σ2,g2)) stat →
+    e2 ∈ t2 →
+    state_interp σ1 (length t1) -∗
+    global_state_interp g1 ncurr mj D (κs ++ κs') -∗
+    wpr CS NotStuck ⊤ e1 r1 Φ Φinv Φr -∗
+    ■ (Φinv -∗ □ Φinv') -∗
+    wptp NotStuck t1 -∗ (* NC 1-∗ *) step_fupdN_fresh ncurr ns (
+      let ntot := (steps_sum num_laters_per_step step_count_next
+                             (Nat.iter (sum_crash_steps ns) step_count_next ncurr )
+                             n)  in
+      let ntot' := ((Nat.iter (n + sum_crash_steps ns) step_count_next ncurr)) in
+      £ (ntot + num_laters_per_step ntot' + 1) -∗
+      (||={⊤|⊤, ∅|∅}=> ||▷=>^ntot ||={∅|∅, ∅|∅}=> ||▷=>^(num_laters_per_step ntot' + 1)
+      ⌜ not_stuck e2 σ2 g2 ⌝)).
+  Proof.
+    intros. destruct stat.
+    - iIntros.
+      iDestruct (wptp_recv_crash_progress with "[$] [$] [$] [$] [$]") as "H"; eauto.
+    - iIntros.
+      iDestruct (wptp_recv_normal_progress with "[$] [$] [$] [$]") as "H"; eauto.
+      iApply (step_fupdN_fresh_wand with "H"); first auto.
+      iIntros "H Hlc".
+      (* iDestruct "H" as (->) "H". *)
+      assert (ns = []) as ->; first by (eapply nrsteps_normal_empty_prefix; eauto).
+      rewrite steps_sum_S_r.
+      simpl. rewrite Nat.add_0_r.
+      iMod ("H" with "[Hlc]") as "H".
+      { iExactEq "Hlc". f_equal. lia. }
+      iModIntro.
+      iApply (step_fupd2N_wand with "H"); auto.
+  Qed.
+
+End recovery_adequacy.
+
+Fixpoint fresh_later_count f g ncurr (ns: list nat) :=
+  match ns with
+  | [] => 0
+  | n :: ns' => S (S (S (crash_adequacy.steps_sum f g ncurr (S n))))
+                 + fresh_later_count f g (Nat.iter (S n) g ncurr) ns'
+  end.
+
+Lemma fresh_later_count_nil f g ncurr :
+  fresh_later_count f g ncurr nil = 0.
+Proof. simpl. lia. Qed.
+Lemma fresh_later_count_cons f g ncurr n (ns': list nat) :
+  fresh_later_count f g ncurr (n::ns') = crash_adequacy.steps_sum f g ncurr (S n) + 3
+                 + fresh_later_count f g (Nat.iter (S n) g ncurr) ns'.
+Proof. simpl. lia. Qed.
+
+Lemma step_fupdN_fresh_rearrange {Λ Σ Ω}
+    `{!irisGS Λ Σ} φ ns ncurr k k2 :
+  (|={⊤}=>
+    step_fupdN_fresh (Ω := Ω) ncurr ns
+      (£ (k + k2) -∗ ||={⊤|⊤,∅|∅}=> ||▷=>^k ||={∅|∅,∅|∅}=> ||▷=>^k2 ⌜φ⌝)) -∗
+  £ (fresh_later_count num_laters_per_step step_count_next ncurr ns + k + k2) -∗
+  ||={⊤|⊤,∅|∅}=> ||▷=>^(fresh_later_count num_laters_per_step step_count_next ncurr ns + S k + k2) ⌜φ⌝.
+Proof.
+  iIntros "H Hlc".
+  iInduction ns as [| n' ns] "IH" forall (ncurr).
+  - rewrite /step_fupdN_fresh.
+    iMod "H". iMod ("H" with "Hlc") as "H". iModIntro.
+    rewrite fresh_later_count_nil.
+    replace (0 + S k) with (k + 1) by lia.
+    rewrite -!assoc -step_fupd2N_add.
+    iApply (step_fupd2N_wand with "H"). iIntros "H".
+    rewrite -step_fupd2N_add.
+    iMod "H". iApply (fupd2_mask_intro); [done..|]. iIntros "_".
+    done.
+  - iMod NC_alloc as (Hc') "HNC".
+    rewrite /step_fupdN_fresh -/step_fupdN_fresh.
+    iMod "H".
+    rewrite fresh_later_count_cons.
+    iEval (rewrite !lc_split -assoc) in "Hlc".
+    iDestruct "Hlc" as "[[[Hlc1 _] Hlc2] Hlck]".
+    iMod ("H" with "Hlc1") as "H". iModIntro.
+    rewrite -!assoc -step_fupd2N_add.
+    iApply (step_fupd2N_wand with "H"). iIntros "H".
+    iApply step_fupd2_fupd2N; first lia.
+    do 2 iMod "H". iModIntro.
+    rewrite -step_fupd2N_add. replace 3 with (2+1) by lia.
+    rewrite -step_fupd2N_add.
+    iApply (step_fupd2N_wand with "H"). iIntros "H".
+    iMod "H".
+Admitted.
+(*     (* iMod "H" as (HG') "H". *) *)
+(*     iMod ("IH" $! with "H [Hlc2 Hlck]") as "H". *)
+(*     { iEval rewrite !lc_split. by iFrame. } *)
+(*     do 3 iModIntro. rewrite assoc. done. *)
+(* Qed. *)
+
+Lemma step_fupdN_fresh_soundness {Λ Σ} {Ω : gGenCmras Σ} `{!invGpreS Σ} `{!crashGpreS Σ} (φ : Prop) ns ncurr k k2 f g:
+  (∀ (Hi: invGS Σ), ⊢ |={⊤}=>
+    ∃ (HI: irisGS Λ Σ) (Hpf1: iris_invGS = Hi)
+     (Hpf2: num_laters_per_step = f) (Hpf2: step_count_next = g),
+      (|={⊤}=> step_fupdN_fresh ncurr ns (
+       £ (k + k2) -∗ ||={⊤|⊤,∅|∅}=> ||▷=>^k ||={∅|∅,∅|∅}=> ||▷=>^k2 ⌜φ⌝))%I) →
+  φ.
+Proof.
+  intros Hiter.
+  eapply (step_fupd2N_soundness (fresh_later_count f g ncurr ns + S k + k2) (fresh_later_count f g ncurr ns + k + k2)).
+  iIntros (Hinv) "Hlc".
+  (* iMod NC_alloc as (Hc) "HNC". *)
+  iMod (Hiter Hinv) as (Hiris <- <- <-) "H".
+  iApply (step_fupdN_fresh_rearrange with "H Hlc").
+Qed.
+
+Record recv_adequate {Λ CS} (s : stuckness) (e1 r1: expr Λ) (σ1 : state Λ) (g1 : global_state Λ)
+    (φ φr: val Λ → state Λ → global_state Λ → Prop) (φinv: state Λ → global_state Λ → Prop)  := {
+  recv_adequate_result_normal t2 σ2 g2 v2 :
+   erased_rsteps (CS := CS) r1 ([e1], (σ1,g1)) (of_val v2 :: t2, (σ2,g2)) Normal →
+   φ v2 σ2 g2;
+  recv_adequate_result_crashed t2 σ2 g2 v2 :
+   erased_rsteps (CS := CS) r1 ([e1], (σ1,g1)) (of_val v2 :: t2, (σ2,g2)) Crashed →
+   φr v2 σ2 g2;
+  recv_adequate_not_stuck t2 σ2 g2 e2 stat :
+   s = NotStuck →
+   erased_rsteps (CS := CS) r1 ([e1], (σ1,g1)) (t2, (σ2,g2)) stat →
+   e2 ∈ t2 → (is_Some (to_val e2) ∨ reducible e2 σ2 g2);
+  recv_adequate_inv t2 σ2 g2 stat :
+   erased_rsteps (CS := CS) r1 ([e1], (σ1,g1)) (t2, (σ2,g2)) stat →
+   φinv σ2 g2
+}.
+
+Lemma recv_adequate_alt {Λ CS} s e1 r1 σ1 g1 (φ φr : val Λ → state Λ → global_state Λ → Prop) φinv :
+  recv_adequate (CS := CS) s e1 r1 σ1 g1 φ φr φinv ↔ ∀ t2 σ2 g2 stat,
+    erased_rsteps (CS := CS) r1 ([e1], (σ1,g1)) (t2, (σ2,g2)) stat →
+      (∀ e2, s = NotStuck → e2 ∈ t2 → (is_Some (to_val e2) ∨ reducible e2 σ2 g2)) ∧
+      (∀ v2 t2', t2 = of_val v2 :: t2' →
+                 match stat with
+                   | Normal => φ v2 σ2 g2
+                   | Crashed => φr v2 σ2 g2
+                 end) ∧
+      (φinv σ2 g2).
+Proof.
+  split.
+  - intros [] ??? []; naive_solver.
+  - constructor; naive_solver.
+Qed.
+
+Corollary wp_recv_adequacy_inv Σ {Ω : gGenCmras Σ} Λ CS
+    `{!invGpreS Σ, !generationGS Λ Σ} nsinit s e r σ g φ φr φinv f1 f2:
+  (∀ `(Hinv : !invGS Σ) `(Hc: !crashGS Σ) κs,
+     ⊢ |={⊤}=> ∃
+         (stateI : state Λ → nat → iProp Σ) (* for the initial generation *)
+         (global_stateI : global_state Λ → nat → fracR → coPset → list (observation Λ) → iProp Σ)
+         (fork_post : val Λ → iProp Σ) Hpf1a Hpf1b
+         Φinv,
+        let HI := IrisGS Λ Σ Hinv (global_stateI) (fork_post) f1 f2 Hpf1a Hpf1b in
+        let HG := GenerationGS Λ Σ Hc stateI in
+       □ (∀ σ nt, stateI σ nt -∗ |={⊤, ∅}=> ⌜ φinv σ ⌝) ∗ (* φinv for initial gen. *)
+       ■ (Φinv Hinv -∗ □ ∀ σ nt, state_interp σ nt -∗ |={⊤, ∅}=> ⌜ φinv σ ⌝) ∗ (* φinv for later generations *)
+       stateI σ 0 ∗ global_stateI g nsinit 1%Qp ∅ κs ∗
+       wpr CS s ⊤ e r (λ v, ⌜φ v⌝) (Φinv Hinv) (λ v, ⌜φr v⌝)) →
+  recv_adequate (CS := CS) s e r σ g (λ v _ _, φ v) (λ v _ _, φr v) (λ σ _, φinv σ).
+Proof.
+  intros Hwp.
+  apply recv_adequate_alt.
+  intros t2 σ2 g2 stat [n [κs H]]%erased_rsteps_nrsteps.
+  (* we apply adequacy twice, for not_stuck and the rest.
+     probably we can somehow avoid all this code duplication... *)
+  split; last first.
+  { destruct (nrsteps_snoc _ _ _ _ _ _ H) as (ns'&n'&->).
+  eapply (step_fupdN_fresh_soundness _ ns' nsinit
+              (crash_adequacy.steps_sum f1 f2 (Nat.iter (sum_crash_steps ns') f2 nsinit) n')
+               (S (S  (f1 (Nat.iter (n' + sum_crash_steps ns') f2 nsinit)))))
+         => Hinv.
+  (* iIntros "HNC". *)
+  iMod (Hwp Hinv _ κs) as (stateI global_stateI fork_post Hpf1a Hpf1b) "H".
+  iDestruct "H" as (Φinv) "(#Hinv1&#Hinv2&Hσ&Hg&H)".
+  iModIntro.
+  set (HI := IrisGS Λ Σ Hinv (global_stateI) (fork_post) f1 f2 Hpf1a Hpf1b).
+  set (HG := GenerationGS Λ Σ _ stateI).
+  iExists HI.
+  iDestruct (wptp_recv_strong_adequacy
+               (Φinv' := (∀ σ nt, state_interp σ nt -∗ |={⊤, ∅}=> ⌜ φinv σ ⌝)%I)
+               (κs' := []) with "[Hσ] [Hg] [H] [] []") as "H"; eauto.
+  { rewrite app_nil_r. eauto. }
+  do 3 iExists eq_refl.
+  iModIntro.
+  iApply (step_fupdN_fresh_wand with "H").
+  { auto. }
+  iIntros "H [Hlc1 Hlc2]".
+  iMod ("H" with "Hlc1") as "H".
+  iApply (step_fupd2N_wand with "H"); auto.
+  iModIntro. iIntros "H".
+  iMod "H" as (v2 ??) "(Hσ&Hg&Hv&Hfpost)".
+  destruct stat.
+  - iDestruct "Hv" as "(Hv&#Hinv)".
+    rewrite ?ncfupd_eq /ncfupd_def.
+    iMod ("Hinv" with "[$]") as "Hp".
+    iApply fupd2_mask_intro; [done..|]. iIntros "_".
+    iApply step_fupd2N_later.
+    repeat iModIntro. iSplit; last done.
+    iIntros (v2' ? Heq). subst. inversion Heq; subst.
+    rewrite to_of_val. naive_solver.
+  -
+    (* iDestruct "Hv" as "(->&Hv)". *)
+    rewrite ?ncfupd_eq /ncfupd_def.
+    iMod ("Hinv1" with "[$]") as "Hp".
+    iApply fupd2_mask_intro; [done..|]. iIntros "_".
+    iApply step_fupd2N_later.
+    repeat iModIntro. iSplit; last done.
+    iIntros (v2' ? Heq). subst. inversion Heq; subst.
+    rewrite to_of_val. naive_solver.
+  }
+  { intros e2 -> He2.
+  destruct (nrsteps_snoc _ _ _ _ _ _ H) as (ns'&n'&->).
+  eapply (step_fupdN_fresh_soundness _ ns' nsinit
+              (crash_adequacy.steps_sum f1 f2 (Nat.iter (sum_crash_steps ns') f2 nsinit) n')
+                (f1 (Nat.iter (n' + sum_crash_steps ns') f2 nsinit) + 1))
+         => Hinv.
+  (* iIntros "HNC". *)
+  iMod (Hwp Hinv _ κs) as (stateI global_stateI fork_post Hpf1a Hpf1b) "H".
+  iDestruct "H" as (Φinv) "(#Hinv1&#Hinv2&Hσ&Hg&H)".
+  iModIntro.
+  set (HI := IrisGS Λ Σ Hinv (global_stateI) (fork_post) f1 f2 Hpf1a Hpf1b).
+  set (HG := GenerationGS Λ Σ _ stateI).
+  iExists HI.
+  (* , HG. *)
+  iDestruct (wptp_recv_progress
+    (Φinv' := (∀ σ nt, state_interp σ nt -∗ |={⊤, ∅}=> ⌜ φinv σ ⌝)%I)
+               (κs' := []) with "[Hσ] [Hg] [H] [] []") as "H"; [eauto..|].
+  { rewrite app_nil_r. eauto. }
+  do 3 iExists eq_refl. iModIntro.
+  iApply (step_fupdN_fresh_wand with "H"); first done.
+  (* iIntros (?). *)
+  iIntros "H Hlc".
+  iApply "H". iExactEq "Hlc". f_equiv; first done.
+  rewrite assoc. f_equiv. done.
+ }
+Qed.
+
